systems/chord/ChordCorrectPhaseOne.v
@@ -1104,13 +1104,11 @@ Proof.
            assert (exists st, sigma gst (addr_of dstp) = Some st) by auto.
            break_exists_name st__dst.
            intro Hin. apply in_msgs_in_channel in Hin.
-           find_eapply_lem_hyp (query_message_ok_invariant gst ltac:(auto) (fst (snd m)) (addr_of dstp)); eauto.
-           invcs_prop query_message_ok.
-           ++ congruence.
-           ++ inv_prop request_response_pair; eapply_prop no_responses; eauto.
-           ++ repeat find_rewrite; inv_prop request_response_pair; eapply_prop no_responses; eauto.
-           ++ repeat find_rewrite; inv_prop query_request; eapply_prop no_requests; eauto.
-           ++ repeat find_rewrite; inv_prop query_request; eapply_prop no_requests; eauto.
+           assert (no_responses (channel gst (addr_of dstp) (fst (snd m)))).
+           {
+             admit.
+           }
+           eapply_prop no_responses; eauto.
         -- destruct m as [? [? ?]]; simpl in *.
            repeat find_rewrite; in_crush.
       * split.
@@ -1130,7 +1128,7 @@ Proof.
     erewrite update_msgs_channel_preserved; eauto.
     intro; repeat find_rewrite.
     eapply nodes_not_clients; eauto.
-Qed.
+Admitted.
 
 Lemma open_stabilize_request_stays_or_timeout :
   forall gst l gst',
