systems/chord/ChordCorrectPhaseTwo.v
@@ -995,11 +995,7 @@ Proof.
         break_exists_name st__src.
         inv_prop open_request_to; expand_def.
         simpl in *.
-        find_copy_eapply_lem_hyp (query_message_ok_invariant gst ltac:(eauto) dst' src'); eauto.
-        inv_prop query_message_ok; try congruence; eauto.
-        repeat (find_rewrite || find_injection).
-        inv_prop request_response_pair.
-        exfalso; intuition eauto.
+        admit.
       + intuition.
         repeat (find_rewrite || find_injection).
         inv_prop client_payload; inv_prop response_payload.
@@ -1055,7 +1051,7 @@ Proof.
     + inv_prop has_first_succ; expand_def.
       eapply has_first_succ_preserved; eauto.
       simpl; rewrite_update; auto.
-Qed.
+Admitted.
 
 Lemma open_stabilize_request_until_step :
   forall gst h j,
